Clean up on Proofs coq file
I cleaned up the file a bit by reorganizing a few things.

src/Proofs.v
@@ -10,24 +10,30 @@ Notation "[ x ; .. ; y ]" := (cons x .. (cons y nil) ..).
 
 
 Inductive simList {X:Type} : nat -> list X -> list X -> Prop :=
-  | simL_eq l1 l2      : forall d, eq l1 l2 -> simList d l1 l2
   | simL_cons h t1 t2  : forall d, simList d t1 t2 
                          -> simList d (cons h t1) (cons h t2)
   | simL_consL h l1 l2 : forall d, simList d l1 l2
                          -> simList (S d) (cons h l1) l2
   | simL_consR h l1 l2 : forall d, simList d l1 l2
-                         -> simList (S d) l1 (cons h l2).
+                         -> simList (S d) l1 (cons h l2)
+  | simL_eq l1 l2      : forall d, eq l1 l2 -> simList d l1 l2.
+
+Lemma simListWeak : forall (X : Type) d (l1 l2 : list X),
+  simList d l1 l2 -> simList (S d) l1 l2.
+Proof. intros X d l1 l2 H.
+  induction H; try (constructor; apply IHsimList).
+  Case "eq". constructor. apply H.
+Qed.
 
 Example simEx1 : simList 1 [1;2] [2].
-Proof. apply simL_consL. apply simL_eq. reflexivity. Qed.
+Proof. constructor. apply simL_eq. reflexivity. Qed.
 
 Example simEx2 : simList 1 [1;2;3;4] [1;3;4].
 Proof. apply simL_cons. 
   apply simL_consL. apply simL_eq. reflexivity. Qed.
 
 Example simEx3 : simList 2 [2] [1].
-Proof. apply simL_consR. apply simL_consL. apply simL_eq. reflexivity. Qed.
-
+Proof. constructor. constructor. constructor. reflexivity. Qed.
 
 Inductive all {X : Type} (P : X -> Prop) : list X -> Prop :=
   | all_nil : all P []
@@ -35,25 +41,23 @@ Inductive all {X : Type} (P : X -> Prop) : list X -> Prop :=
 
 
 Inductive simNat : nat -> nat -> nat -> Prop :=
-  | simN_eq n1 n2   : forall d, eq_nat n1 n2 -> simNat d n1 n2
   | simN_S n1 n2    : forall d, simNat d n1 n2 -> simNat d (S n1) (S n2)
   | simN_l n1 n2    : forall d, simNat d n1 n2 -> simNat (S d) (S n1) n2
-  | simN_r n1 n2    : forall d, simNat d n1 n2 -> simNat (S d) n1 (S n2).
+  | simN_r n1 n2    : forall d, simNat d n1 n2 -> simNat (S d) n1 (S n2)
+  | simN_eq n1 n2   : forall d, eq_nat n1 n2 -> simNat d n1 n2.
 
 Lemma simNatPlus : forall (d n s1 s2 : nat),
   simNat d s1 s2 -> simNat d (n+s1) (n+s2).
 Proof. intros d n s1 s2 H. induction n as [| n' IHn].
   simpl. apply H.
-  simpl. apply simN_S. apply IHn.
+  simpl. constructor. apply IHn.
 Qed.
 
 Lemma simNatWeak : forall d n1 n2,
   simNat d n1 n2 -> simNat (S d) n1 n2.
-Proof. intros d n1 n2 H. induction H.
-  Case "eq". apply simN_eq. apply H.
-  Case "S". apply simN_S. apply IHsimNat.
-  Case "l". apply simN_l. apply IHsimNat.
-  Case "r". apply simN_r. apply IHsimNat.
+Proof. intros d n1 n2 H.
+  induction H; try (constructor; apply IHsimNat).
+  Case "eq". constructor. apply H.
 Qed.
 
 
@@ -74,12 +78,10 @@ Lemma foo : forall (Arg Arg' : list nat) (d:nat),
   all (fun x => x <= 1) Arg' ->
   simNat d (sumList Arg) (sumList Arg').
 Proof. intros Arg Arg' d HListSim HArgClip HArg'Clip.
-induction HListSim as [l1 l2 d eq |
+induction HListSim as [h l1 l2 d HListSim' IHLS|
                        h l1 l2 d HListSim' IHLS|
                        h l1 l2 d HListSim' IHLS|
-                       h l1 l2 d HListSim' IHLS].
-  Case "eq".
-    rewrite eq. apply simN_eq. apply eq_nat_refl.
+                       l1 l2 d eq].
   Case "cons".
     simpl. apply simNatPlus. apply IHLS.
     inversion HArgClip as [ | x l HLT1 HLTTail].
@@ -90,7 +92,7 @@ induction HListSim as [l1 l2 d eq |
     inversion HArgClip as [asdf | x l HLT1 HLTTail].
     inversion HLT1 as [ | x' HLT0].
     SCase "head is 1".
-      simpl. apply simN_l. apply IHLS.
+      simpl. constructor. apply IHLS.
       apply HLTTail. apply HArg'Clip.
     SCase "head is 0".
       inversion HLT0.
@@ -100,12 +102,14 @@ induction HListSim as [l1 l2 d eq |
     inversion HArg'Clip as [ | x l HLT1 HLTTail].
     inversion HLT1 as [ | x' HLT0].
     SCase "head is 1".
-      simpl. apply simN_r. apply IHLS.
+      simpl. constructor. apply IHLS.
       apply HArgClip. apply HLTTail.
     SCase "head is 0".
       inversion HLT0.
       simpl. apply simNatWeak. apply IHLS.
         apply HArgClip. apply HLTTail.
+  Case "eq".
+    rewrite eq. constructor. apply eq_nat_refl.
 Qed.
     
 
